finished initial dump

allSatisfyingExample.py
@@ -1,0 +1,72 @@
+
+from z3 import *
+import sys
+
+print(sys.setrecursionlimit(1000))
+COUNT = 0
+
+
+def all_smt(s, initial_terms):
+    def block_term(s, m, t):
+        # print("blocking : " + str(t != m.eval(t, model_completion=True)))
+        s.add(t != m.eval(t, model_completion=True))
+    def fix_term(s, m, t):
+        # print("fixing : " + str(t == m.eval(t, model_completion=True)))
+        s.add(t == m.eval(t, model_completion=True))
+    def all_smt_rec(terms):
+        global COUNT
+        if sat == s.check():
+           m = s.model()
+           yield m
+        #    print(m)
+        #    print("here " + str(COUNT))
+           COUNT = COUNT + 1
+        #    if(COUNT == 1000):
+        #     return None
+           for i in range(len(terms)):
+               s.push()
+               block_term(s, m, terms[i])
+               for j in range(i):
+                   fix_term(s, m, terms[j])
+               yield from all_smt_rec(terms[i:])
+               s.pop()   
+
+    yield from all_smt_rec(list(initial_terms))
+
+
+x = Int('x')
+y = Int('y')
+s = Solver()
+v = x + y < 10, x > 1, y > 1
+s.add(v)
+print(s.check())
+print(s.model())
+
+models = list(all_smt(s,[x,y]))
+# print (len(models))
+print ((models))
+
+a = Int('a')
+b = Int('b')
+c = Int('c')
+s = Solver()
+
+s.add(And(c >= a, c >= b),a >= 0,a < 10,b >= 0,b < 10,c < 50)
+vals = list(all_smt(s, [a, b,c]))[:100]
+
+for i in range (len(vals)):
+    print(""+str(i) + " :: " + str(vals[i]))
+# print(vals)
+# aVals = "["
+# bVals = "["
+# cVals = "["
+# for x in vals:
+#     aVals = aVals + str(x[a]) + ","
+#     bVals = bVals + str(x[b]) + ","
+#     cVals = cVals + str(x[c]) + ","
+# print(aVals)
+# print("---")
+# print(bVals)
+# print("---")
+# print(cVals)
+# print("---")
