fuzzingSimple.py
@@ -1,0 +1,451 @@
+
+#!/usr/bin/python
+import sys, getopt
+from z3 import *
+import json
+
+print(sys.setrecursionlimit(1000))
+COUNT = 0
+
+
+
+
+def all_smt(s, initial_terms,bound,count):
+    listTest = []
+    COUNT = 0
+    def block_term(s, m, t):
+        # print("blocking : " + str(t != m.eval(t, model_completion=True)))
+        s.add(t != m.eval(t, model_completion=True))
+    def fix_term(s, m, t):
+        # print("fixing : " + str(t == m.eval(t, model_completion=True)))
+        s.add(t == m.eval(t, model_completion=True))
+    def all_smt_rec(terms,bound,c):
+        global COUNT
+        if sat == s.check():
+           m = s.model()
+           yield m
+           listTest.append(m)
+        #    print("M == " ,listTest)
+        #    print("here " + str(c))
+           c = c + 1
+           if(c >= bound):
+             raise Exception("Current val at bound",listTest)
+    
+           for i in range(len(terms)):
+            #    print(i)
+               s.push()
+               block_term(s, m, terms[i])
+            #    print("afterBlock")
+               for j in range(i):
+                   fix_term(s, m, terms[j])
+            #    print("TERMS = " , terms[i:])
+            #    print("S == ", s)
+               yield from all_smt_rec(terms[i:],bound,c)
+            #    print("S POP !! == ", s)
+               s.pop()   
+
+    yield from all_smt_rec(list(initial_terms),bound,count)
+
+
+x = Int('x')
+y = Int('y')
+s = Solver()
+# v = x + y < 10, x > 1, y > 1
+v = x + y < 10
+
+s.add(v)
+# print(s.check())
+# print(s.model())
+try:
+    models = list(all_smt(s,[x,y],4,0))
+except Exception as e:
+    # print(e)
+    msg,models = e.args
+
+print (len(models))
+for m in models:
+    print(m)
+print ((models))
+
+print("++++++")
+x = Int('x')
+y = Int('y')
+s = Solver()
+v =  eval("x + y < 10, x > 1, y > 1")
+print(v)
+s.add(v)
+# print(s.check())
+# print(s.model())
+
+# models = list(bounded_smt_rec(s,[x,y],10))
+# print (len(models))
+# print ((models))
+
+a = Int('a')
+b = Int('b')
+c = Int('c')
+s = Solver()
+
+# s.add(And(c >= a, c >= b),a >= 0,a < 10,b >= 0,b < 10,c < 50)
+s.add(And(c >= a, c >= b), Or(c == a, c == b))
+# print simplify(And(c >= a, c >= b), Or(c == a, c == b))
+# s.add(And(c >= a, c >= b),a >= 0,a < 10,b >= 0,b < 10,c < 50)
+
+# vals = list(all_smt(s, [a, b,c]))
+try:
+    models = list(all_smt(s,[a,b,c],10,0))
+except Exception as e:
+    print(e)
+    msg,models = e.args
+
+# print (len(models))
+for m in models:
+    print(m)
+
+
+x = Int('x')
+y = Int('y')
+n = x + y >= 3
+print("num args: ", n.num_args())
+print("children: ", n.children())
+print("1st child:", n.arg(0))
+print("2nd child:", n.arg(1))
+print("operator: ", n.decl())
+print("op name:  ", n.decl().name())
+
+listofVars = ["a"]
+_a = locals()
+for v in listofVars:
+    _a[v] = Int(str(v))
+    print( _a[v])
+# f = Function('f', IntSort(), IntSort(), IntSort())
+# /////
+#works with predicates right now
+def findFunctionInFile(in_filename,origFnName):
+    fo = open(in_filename,"r+")
+    dafnyCode = fo.readlines()
+    count = 0
+    listofLines = []
+    foundStart = False
+    # Look for a predicate
+    fullFnName = "predicate "+ origFnName + "("
+    for line in dafnyCode:
+        args = line.split()
+        if(foundStart and line.strip()):   
+            listofLines.append(line.strip())
+        else:
+            foundStart = False
+        if(fullFnName in line):
+            listofLines.append(line.strip())
+            foundStart = True
+        count = count + 1
+    if (listofLines == []):
+        #could be a lemma!
+        count = 0
+        fullFnName = "lemma "+ origFnName + "("
+        for line in dafnyCode:
+            args = line.split()
+            if(foundStart and line.strip()):   
+                listofLines.append(line.strip())
+            else:
+                foundStart = False
+            if(fullFnName in line):
+                listofLines.append(line.strip())
+                foundStart = True
+            count = count + 1
+    return listofLines
+
+#returns
+# (parameterMap) == map of parameters to their
+def stripParameterTypes(parameterList):
+    parameterMap = {}
+    for p in parameterList:
+        splitP = p.split(":")
+        parameterMap[splitP[0]] = splitP[1]
+    return(parameterMap)
+
+def parsePredicateBody(functionTxt):
+    body = functionTxt[2:-1]
+    
+    print(body)
+
+def createSMTQuery(vals,query,numOfTrials):
+    listofVars = []
+    _g = globals()
+    for v in vals:
+        if(vals.get(v) == "Int"):
+            temp = Int(str(v))
+            listofVars.append(temp)
+    print(listofVars) 
+    s = Solver()
+    v =  eval(query)
+    s.add(v)
+
+    try:
+        models = list(all_smt(s,[a,b,c],int(numOfTrials),0))
+    except Exception as e:
+    # print(e)
+        msg,models = e.args
+    for m in models:
+        print(m)
+    #MAX
+    for var in listofVars:
+        s = Solver()
+        v =  eval(query)
+        s.add(v)
+        print("====Testing MAX Values for: ", var,"======")
+        s.add(var == sys.maxsize)
+        print(s)
+        try:
+            models = list(all_smt(s,listofVars,2,0))
+        except Exception as e:
+            msg,models = e.args
+        for m in models:
+            print(m)
+    #MIN
+    for var in listofVars:
+        s = Solver()
+        v =  eval(query)
+        s.add(v)
+        print("====Testing MIN Values for: ", var,"======")
+        s.add(var == -sys.maxsize-1)
+        print(s)
+        try:
+            models = list(all_smt(s,listofVars,2,0))
+        except Exception as e:
+            msg,models = e.args
+        for m in models:
+            print(m)
+
+
+def usage():
+    return ("fuzzing.py" + 
+                    "\n\t -vals [dictionary of input type pairs] " +
+                    "\n\t\t i.e:  '{ \"key1\": \"value 1\", \"key2\": \"value 2\" }' " + 
+                    "\n\t -q <query> "+ 
+                    "\n\t\t smt query i.e: \"And(c >= a, c >= b), Or(c == a, c == b)\"")
+def maxTest(a, b, c):
+    val: bool = False
+    val = ((c) > (a)) and ((c) > (b))
+    return val
+
+
+def main(argv):
+    vals = {}
+    query = ""
+    numOfTrials = 0
+    try:
+        opts, args = getopt.getopt(argv,"hi:q:v:n:",["vals=","query=","numOfTrials="])
+    except getopt.GetoptError:
+        print(usage())
+        sys.exit(2)
+    for opt, arg in opts:
+        if opt == '-h':
+            print(usage())
+            sys.exit()
+        elif opt in ("-v", "--vals"):
+            vals = json.loads(arg)
+        elif opt in ("-q", "--query"):
+            query = arg
+        elif opt in ("-n", "--numOfTrials"):
+            numOfTrials = arg
+
+    print("======================================")
+    print('vals are: ', json.dumps(vals))
+    print('query is: ', query)
+    print('num of trials: ', numOfTrials)
+    print("======================================")
+    createSMTQuery(vals,query,numOfTrials) #ASSUMES ALL VAR ARE INT
+    # for a in vals:
+    #     print(vals.get(a))
+
+
+if __name__ == "__main__":
+   main(sys.argv[1:])
+
+
+# def main(argv):
+#     inputfile = ''
+#     nameOfFunction = ''
+#     smFlag = False
+#     try:
+#         opts, args = getopt.getopt(argv,"hi:n:s:",["ifile=","noffun=","smFlag="])
+#     except getopt.GetoptError:
+#         print(usage())
+#         sys.exit(2)
+#     for opt, arg in opts:
+#         if opt == '-h':
+#             print(usage())
+#             sys.exit()
+#         elif opt in ("-i", "--ifile"):
+#             inputfile = arg
+#         elif opt in ("-n", "--noffun"):
+#             nameOfFunction = arg
+#         elif opt in ("-s", "--smFlag"):
+#             smFlag = arg
+#     print("======================================")
+#     print('Input file is: ', inputfile)
+#     print('Name of Function to test is: ', nameOfFunction)
+#     print('StateMachineFlag: ', smFlag)
+#     print("======================================\n")
+    
+#     functionTxt = findFunctionInFile(inputfile,nameOfFunction)
+#     print(functionTxt)
+#     if(functionTxt[0].split()[0] == "predicate"):
+#         parameters = functionTxt[0].split("(")[1][:-1].split(",")
+#         pMap = stripParameterTypes(parameters)
+#         print(pMap)
+#         parsePredicateBody(functionTxt)
+#         print(maxTest(1,2,3))
+#     else:
+#         print("INPUT not correct")
+#     print("DONE")
+
+# ASSUME THAT INPUT IS PREDICATE IN FORM:
+
+# Predicate Name(parameters)
+# {
+#     && (clause || clause) 
+#     && clause
+#     || clause
+# }
+# // === OLD iterative trial
+
+# def bounded_block_term(s, m, t):
+#         print("blocking : " + str(t != m.eval(t, model_completion=True)))
+#         s.add(t != m.eval(t, model_completion=True))
+
+# def bounded_fix_term(s, m, t):
+#         print("fixing : " + str(t == m.eval(t, model_completion=True)))
+#         s.add(t == m.eval(t, model_completion=True))
+
+# def bounded_smt_rec(s,terms,bound):
+#     listOfSmtResults = []
+#     if sat == s.check():
+#            m = s.model()
+#            listOfSmtResults.append(m)
+#            i = 0
+#            while(len(listOfSmtResults) < bound):
+#             print("i  = " + str(i) + " :: " + str(s))
+#             if(i >= len(terms)):
+#                 # i = 0
+#                 return  listOfSmtResults
+#                 # terms = terms[1:]
+#             print("i  = " + str(i) + " :: " + str(terms))
+
+#             s.push()
+#             bounded_block_term(s, m, terms[i])
+#             for j in range(i):
+#                 bounded_fix_term(s, m, terms[j])
+#             if sat == s.check():
+#                 m = s.model()
+#                 listOfSmtResults.append(m)
+#                 print("ERE " + str(m) + "len = " + str(len(listOfSmtResults)))
+#                 print(s)
+                
+#             else:
+#                 print("inc I")
+#                 s.pop()
+#                 i += 1
+#            return  listOfSmtResults
+
+# def bounded_smt_rec_v2(s,terms,bound,listOfSmtResults):
+#     i = 0
+#     termIndex = 0
+#     pushCount = 1
+#     while(len(listOfSmtResults) < bound and termIndex < len(terms)):
+#         if sat == s.check():
+#             m = s.model()
+#             listOfSmtResults.append(m)
+#             # for i in range(len(terms)):
+#             s.push()
+#             bounded_block_term(s, m, terms[termIndex])
+#             for j in range(termIndex):
+#                 bounded_fix_term(s, m, terms[j])
+#             # listOfSmtResults.append(bounded_smt_rec_v2(s,terms[termIndex:],bound,listOfSmtResults))
+#         else:
+#             # print("HERE == ", s)
+#             for popCount in range(pushCount):
+#                 s.pop()
+#             pushCount += 1
+#             termIndex += 1
+#             i += 1
+#     return listOfSmtResults
+
+
+
+# ////
+# x = Int('x')
+# y = Int('y')
+# s = Solver()
+# # v = x + y < 10, x > 1, y > 1
+# v = x + y < 10
+
+# s.add(v)
+# # print(s.check())
+# # print(s.model())
+# try:
+#     models = list(all_smt(s,[x,y],4,0))
+# except Exception as e:
+#     # print(e)
+#     msg,models = e.args
+
+# print (len(models))
+# for m in models:
+#     print(m)
+# print ((models))
+
+# print("++++++")
+# x = Int('x')
+# y = Int('y')
+# s = Solver()
+# v =  eval("x + y < 10, x > 1, y > 1")
+# print(v)
+# s.add(v)
+# # print(s.check())
+# # print(s.model())
+
+# # models = list(bounded_smt_rec(s,[x,y],10))
+# # print (len(models))
+# # print ((models))
+
+# a = Int('a')
+# b = Int('b')
+# c = Int('c')
+# s = Solver()
+
+# # s.add(And(c >= a, c >= b),a >= 0,a < 10,b >= 0,b < 10,c < 50)
+# s.add(And(c >= a, c >= b), Or(c == a, c == b))
+# # print simplify(And(c >= a, c >= b), Or(c == a, c == b))
+# # s.add(And(c >= a, c >= b),a >= 0,a < 10,b >= 0,b < 10,c < 50)
+
+# # vals = list(all_smt(s, [a, b,c]))
+# try:
+#     models = list(all_smt(s,[a,b,c],10,0))
+# except Exception as e:
+#     print(e)
+#     msg,models = e.args
+
+# # print (len(models))
+# for m in models:
+#     print(m)
+
+
+# c = Int('c')
+# v = Int('v')
+# w = Int('w')
+# s = Solver()
+
+# v = eval("And(v >= 0, v <= c, v > 0, w == v - 1)")
+# print("!!!!!! = " ,v)
+
+# s.add(v)
+# print(s.check())
+# print(s.model())
+# print(s.check())
+# print(s.model())
+# listOfVars = ["a"]
+# _a = locals()
+# for v in listOfVars:
+#     _a[v] = Int(str(v))
+#     print( _a[v])
