test.py
@@ -1,0 +1,259 @@
+
+from z3 import *
+import sys
+# from mpl_toolkits import mplot3d
+import numpy as np
+# import matplotlib.pyplot as plt
+
+print(sys.setrecursionlimit(1000))
+
+COUNT = 0
+# count = 0
+
+
+def fullMaxSpec(o):
+    return And(o >= a, o >= b, Or(o == b, o == a))
+
+def partialMaxSpec(o):
+    return And(o >= a, o >= b)
+
+
+def tooStrongMax(o):
+    return And(o > a, o > b, Or(o == b, o == a))
+
+def between(o):
+    return And(o >= a, o <= b) 
+
+def test_smt(s,initial_terms):
+    def block_term(s, m, t):
+        global COUNT
+        print("blocking1 : "+ str(COUNT) + " " + str(t != m.eval(t, model_completion=True)))
+        s.add(t != m.eval(t, model_completion=True))
+        COUNT = COUNT + 1
+        if(COUNT >= 2):
+            return None
+    def fix_term(s, m, t, i):
+        for j in range(i):
+            print("fixing : " + str(t[j] == m.eval(t[j], model_completion=True)))
+            s.add(t[j] == m.eval(t[j], model_completion=True))
+    def test_smt_rec(terms):
+        # global COUNT
+        if sat == s.check():
+           m = s.model()
+           yield m
+           i = len(terms)-1
+        #    for i in range(len(terms)):
+           s.push()
+           block_term(s, m, terms[i])
+           fix_term(s, m, terms,i)
+           yield from test_smt_rec(terms[i:])
+           s.pop()   
+        #    for j in range(i):
+        #     fix_term(s, m, terms[j])
+        #     yield from test_smt_rec(terms[i:])
+        #     s.pop()   
+    yield from test_smt_rec(list(initial_terms))
+
+
+print ("--Random Spec--")
+
+x = Int('x')
+y = Int('y')
+s = Solver()
+v = x + y < 10, x > 1, y > 1
+s.add(v)
+print(s.check())
+print(s.model())
+# simple Test
+
+terms = [x,y]
+
+m = s.model()
+s_diff = Solver()
+s_diff.add(v)
+for i in range(len(terms)-1):
+    print ("fixing (input) = " + str(terms[i]))
+    s_diff.add(terms[i] == m.eval(terms[i], model_completion=True)) #ask input to be the same
+print ("blocking previous result for = " + str(terms[len(terms)-1]))
+s_diff.add(terms[len(terms)-1] != m.eval(terms[len(terms)-1], model_completion=True)) #ask output to be different
+check = s_diff.check()
+print(check)
+if (check == sat):
+    print(s_diff.model())
+else:
+    print("unsat")
+# models = list(test_smt(s,[x,y]))
+# print (len(models))
+# print ((models))
+
+print ("--Incomplete Max Spec--")
+
+
+a = Int('a')
+b = Int('b')
+c = Int('c')
+s = Solver()
+v = And(c >= a, c >= b)
+# s.add(a == 6)
+s.add(v)
+print(s.check())
+print(s.model())
+
+terms = [a,b,c]
+m = s.model()
+s_diff = Solver()
+s_diff.add(v)
+for i in range(len(terms)-1):
+    print ("fixing (input) = " + str(terms[i]))
+    s_diff.add(terms[i] == m.eval(terms[i], model_completion=True)) #ask input to be the same
+print ("blocking previous result for = " + str(terms[len(terms)-1]))
+s_diff.add(terms[len(terms)-1] != m.eval(terms[len(terms)-1], model_completion=True)) #ask output to be different
+check = s_diff.check()
+print(check)
+if (check == sat):
+    print(s_diff.model())
+else:
+    print("unsat")
+
+
+print ("--Complete Max Spec--")
+
+
+a = Int('a')
+b = Int('b')
+c = Int('c')
+s = Solver()
+v = And(c >= a, c >= b, Or(c == b, c == a))
+s.add(v)
+print(s.check())
+print(s.model())
+
+terms = [a,b,c]
+m = s.model()
+s_diff = Solver()
+s_diff.add(v)
+for i in range(len(terms)-1):
+    print ("fixing (input) = " + str(terms[i]))
+    s_diff.add(terms[i] == m.eval(terms[i], model_completion=True)) #ask input to be the same
+print ("blocking previous result for = " + str(terms[len(terms)-1]))
+s_diff.add(terms[len(terms)-1] != m.eval(terms[len(terms)-1], model_completion=True)) #ask output to be different
+check = s_diff.check()
+print(check)
+if (check == sat):
+    print(s_diff.model())
+else:
+    print("unsat")
+
+
+print ("--test full--")
+
+a = Int('a')
+b = Int('b')
+c = Int('c')
+d = Int('d')
+s = Solver()
+
+s.add(fullMaxSpec(c))
+s.add(d != c)
+s.add(fullMaxSpec(d)) 
+
+check = s.check()
+print(check)
+if (check == sat):
+    print(s.model())
+else:
+    print("unsat")
+
+
+print ("--test partial--")
+
+a = Int('a')
+b = Int('b')
+c = Int('c')
+d = Int('d')
+s = Solver()
+
+s.add(And(c >= a, c >= b))
+s.add(d != c)
+s.add(And(d >= a, d >= b))
+
+s.add(partialMaxSpec(c))
+s.add(d != c)
+s.add(partialMaxSpec(d)) 
+
+check = s.check()
+print(check)
+if (check == sat):
+    print(s.model())
+else:
+    print("unsat")
+
+
+print ("--test full--")
+
+a = Int('a') 
+b = Int('b')
+c = Int('c')
+d = Int('d')
+s = Solver()
+
+
+s.add(fullMaxSpec(c))
+s.add(d != c)
+s.add(fullMaxSpec(d)) 
+
+check = s.check()
+print(check)
+if (check == sat):
+    print(s.model())
+else:
+    print("unsat")
+
+
+print ("--test too strong--")
+
+a = Int('a')
+b = Int('b')
+c = Int('c')
+d = Int('d')
+s = Solver()
+
+s.add(tooStrongMax(c))
+# s.add(d != c)
+# s.add(partialMaxSpec(d)) 
+
+check = s.check()
+print(check)
+if (check == sat):
+    print(s.model())
+else:
+    print("unsat")
+
+# print ("--Sort Spec--")
+
+# s = Solver()
+
+# # Use I as an alias for IntSort()
+# I = IntSort()
+# # A is an array from integer to integer
+# A = Array('A', I, I)
+# B = Array('B', I, I)
+
+# length = Int('length')
+# x = Int('x')
+# y = Int('y')
+# print (A[x])
+# # print (Select(A, x))
+# # print (Store(A, x, 10))
+# # print (simplify(Select(Store(A, 2, x+1), 2)))
+
+# # s.add(And(A[0] > 10,A[1] < A[0],A[2] < A[1],A[2]> 0))
+# v = ForAll(x,Implies(And(x >= 0, x < (length - 1) ),And(B[x] <= B[x+1])))
+# vv = ForAll(x,Implies(And(x >= 0, x < length),Exists (y,A[y] == B[x])))
+# greaterThanZero = length > 2
+# s.add(greaterThanZero)
+# s.add(v)
+# s.add(vv)
+# s.add(B[0] <= B[1])
+# print(s.check())
+# print(s.model())
