template.s.dfy
@@ -1,53 +1,72 @@
+
+
+
 datatype Constants = Constants(capacity:int)
 datatype CokeMachine = CokeMachine(numCokes:int)
 
-
-predicate pred<T(==)>(a:T,b:T)
+predicate  predMaxEx(a:int,b:int,c:int)
 {
-    a == b
-}
+  && c > a
+  && c >= b
+} 
 
-predicate divides(factor:nat, candidate:nat)
-  requires 1<=factor
-{
-  candidate % factor == 0
-}
+// predicate pred<T(==)>(a:T,b:T)
+// {
+//     a == b
+// }
 
-predicate StateTrans<C,V>(c:C,v:V,v':V)
-{
-  true
-}
+// predicate divides(factor:nat, candidate:nat)
+//   requires 1<=factor
+// {
+//   candidate % factor == 0
+// }
 
-lemma isPredSM_ND<C,V>(c:C,v:V,v':V,v'':V)
-  requires StateTrans(c,v,v')
-  requires StateTrans(c,v,v'')
-//   ensures v' == v''
-//   {}
+// predicate StateTrans<C,V>(c:C,v:V,v':V)
+// {
+//   true
+// }
 
-predicate Purchase(c:Constants, v:CokeMachine, v':CokeMachine) 
-{
-    && v.numCokes > 0
-    && v'.numCokes == v.numCokes - 1
-}
+// lemma isPredSM_ND<C,V>(c:C,v:V,v':V,v'':V)
+//   requires StateTrans(c,v,v')
+//   requires StateTrans(c,v,v'')
+// //   ensures v' == v''
+// //   {}
 
-predicate PurchaseND(c:Constants, v:CokeMachine, v':CokeMachine) 
-{
-    && v.numCokes > 0
-    && v'.numCokes <= v.numCokes - 1
-}
+// predicate Purchase(c:Constants, v:CokeMachine, v':CokeMachine) 
+// {
+//     && v.numCokes > 0
+//     && v'.numCokes == v.numCokes - 1
+// }
 
-predicate pre<T>(a:T){
-	true
-}
+// predicate PurchaseND(c:Constants, v:CokeMachine, v':CokeMachine) 
+// {
+//     && v.numCokes > 0
+//     && v'.numCokes <= v.numCokes - 1
+// }
 
-predicate post<T>(a:T){
-	true
-}
+// predicate pre<T>(a:T){
+// 	true
+// }
 
-lemma maxExample(a:int,b:int) returns (c:int)
+// predicate post<T>(a:T){
+// 	true
+// }
+
+
+
+lemma {:extern} maxExample(a:int,b:int) returns (c:int)
 	requires a > 0
-  ensures c > a
+  	ensures c > a
 	ensures c > b
+
+
+// lemma is_maxExample_ND(a:int,b:int)
+//         requires a > 0
+// {
+//         var result := maxExample(a,b);
+//         var result' := maxExample(a,b);
+//         assert result == result';
+// }
 
 lemma maxExampleD(a:int,b:int) returns (c:int)
 	ensures c >= a
@@ -61,38 +80,38 @@ lemma is_maxExampleD_ND(a:int,b:int)
         assert result == result';
 }
 
-lemma isMaxExampleNDD(a:int,b:int)
-{
-	var c := maxExampleD(a,b);
-	var c' := maxExampleD(a,b);
-	assert c == c';
-}
+// lemma isMaxExampleNDD(a:int,b:int)
+// {
+// 	var c := maxExampleD(a,b);
+// 	var c' := maxExampleD(a,b);
+// 	assert c == c';
+// }
 
-lemma lemmaOrMethodThatReturnsAValue<T>(a:T) returns (b:T)
-    requires pre(a)
-    ensures post(b)
+// lemma lemmaOrMethodThatReturnsAValue<T>(a:T) returns (b:T)
+//     requires pre(a)
+//     ensures post(b)
 
-  lemma isLemmaND<T>(a:T,a':T) returns (result:bool)
-    requires pre(a) && pre(a')
-    requires a == a'
-    // ensures result
-  {
-    var b := lemmaOrMethodThatReturnsAValue(a);
-    var b' := lemmaOrMethodThatReturnsAValue(a');
-    // return b == b';
-  }
+//   lemma isLemmaND<T>(a:T,a':T) returns (result:bool)
+//     requires pre(a) && pre(a')
+//     requires a == a'
+//     // ensures result
+//   {
+//     var b := lemmaOrMethodThatReturnsAValue(a);
+//     var b' := lemmaOrMethodThatReturnsAValue(a');
+//     // return b == b';
+//   }
 
-    predicate convertedPredicate<T>(a:T,b:T)
-    requires pre(a)
-  {
-    post(b)
+//     predicate convertedPredicate<T>(a:T,b:T)
+//     requires pre(a)
+//   {
+//     post(b)
 
-  }
+//   }
 
-    lemma isConvertedLemmaorMethodND<T>(a:T,b:T,b':T)
-    requires pre(a)
-    requires convertedPredicate(a,b)
-    requires convertedPredicate(a,b')
-    // ensures b == b'
-    // {}
+//     lemma isConvertedLemmaorMethodND<T>(a:T,b:T,b':T)
+//     requires pre(a)
+//     requires convertedPredicate(a,b)
+//     requires convertedPredicate(a,b')
+//     // ensures b == b'
+//     // {}
   
