leaderTest.s.dfy
@@ -1,121 +1,65 @@
-module leader 
+module leader
 {
-
-datatype agent = Ldr | Acc
-
-datatype Id = Id(agt:agent, idx:nat)
-
-datatype Value = V(val:int) | Nil
-datatype Ballot = Ballot(seqNo:nat, idx:nat) | Bottom
-datatype ValBal = VB(v:Value, b:Ballot)
-
-datatype Message = Prepare(bal:Ballot)
-                | Promise(bal:Ballot, vb:ValBal)  //valbal is the value-ballot pair with which the value was accepted
-                | Propose(bal:Ballot, val:Value)
-                | Accept(bal:Ballot, val:Value)
-                | Preempt(bal:Ballot)
-
-datatype Packet = Packet(src:Id, dst:Id, msg:Message)
-
-datatype EnvStep = 
-    IoStep(actor:Id, recvIos:seq<Packet>, sendIos:seq<Packet>)
-
-datatype Environment = Env(
-        sentPackets:set<Packet>,
-        nextStep:EnvStep
-    )
-
-predicate EnvironmentInit(e:Environment) {
-    e.sentPackets == {}
-}
-
-predicate ValidIoStep(iostep:EnvStep) 
-    requires iostep.IoStep?
-{
-    && (forall r | r in iostep.recvIos :: r.dst == iostep.actor)
-    && (forall s | s in iostep.sendIos :: s.src == iostep.actor)
-}
-
-
-predicate EnvironmentNext(e:Environment, e':Environment)
-{
-    match e.nextStep {
-        case IoStep(actor, recvIos, sendIos) => 
-            && ValidIoStep(e.nextStep)
-            && e'.sentPackets == e.sentPackets + (set s | s in sendIos)
-            && e'.nextStep == e.nextStep
-            && (forall r | r in recvIos :: r in e.sentPackets)
-    }
-}
-
-lemma testN(a:Environment) returns (a':Environment,b:Environment)
-    ensures !(EnvironmentNext(a,a') 
-              && a' != b
-              && EnvironmentNext(a,b))
-{
-
-}
-
 // Each node's identifier (address)
 datatype Constants = Constants(ids: seq<nat>) {
     predicate ValidIdx(i: nat) {
-        0<=i<|ids|
-    }
-    predicate UniqueIds() {
-        (forall i:nat, j:nat | ValidIdx(i) && ValidIdx(j) && ids[i]==ids[j] :: i == j)
-    } 
-    predicate WF() {
-        0 < |ids|
-    }
-}
+            0<=i<|ids|
+	        }
+		    predicate UniqueIds() {
+		            (forall i:nat, j:nat | ValidIdx(i) && ValidIdx(j) && ids[i]==ids[j] :: i == j)
+			        }
+				    predicate WF() {
+				            0 < |ids|
+					        }
+						}
 
 
 // The highest other identifier this node has heard about.
 datatype Variables = Variables(highest_heard: seq<nat>) {
     predicate WF(c: Constants)
-        requires c.WF()
-    {
-        && |highest_heard| == |c.ids|
-    }
-}
+            requires c.WF()
+	        {
+		        && |highest_heard| == |c.ids|
+			    }
+			    }
 
 function NextIdx(c:Constants, idx:nat) : (n:nat)
   requires c.WF()
-  requires c.ValidIdx(idx)
-  ensures n == 0 || n == idx + 1
-  ensures idx == |c.ids| - 1 <==> n == 0 
-  ensures idx < |c.ids| - 1 <==> n == idx + 1
-{
-    (idx + 1) % |c.ids|
-}
+    requires c.ValidIdx(idx)
+      ensures n == 0 || n == idx + 1
+        ensures idx == |c.ids| - 1 <==> n == 0
+	  ensures idx < |c.ids| - 1 <==> n == idx + 1
+	  {
+	      (idx + 1) % |c.ids|
+	      }
 
 function max(a:nat, b:nat) : nat {
     if a > b then a else b
-}
+    }
 
 predicate Transmission(c: Constants, v: Variables, v': Variables, src: nat)
 {
     && c.WF()
-    && v.WF(c)
-    && v'.WF(c)
-    && c.ValidIdx(src)
-    // Neighbor address in ring.
-    && var dst := NextIdx(c, src);
-    // src sends the max of its highest_heard value and its own id.
-    && var message := max(v.highest_heard[src], c.ids[src]);
-    // dst only overwrites its highest_heard if the message is higher.
-    && var dst_new_max := max(v.highest_heard[dst], message);
-    // && v' == v.(highest_heard := v.highest_heard[dst := message])  // BUG: dst := dst_new_max
-    && v' == v.(highest_heard := v.highest_heard[dst := dst_new_max])
-}
+        && v.WF(c)
+	    && v'.WF(c)
+	        && c.ValidIdx(src)
+		    // Neighbor address in ring.
+		        && var dst := NextIdx(c, src);
+			    // src sends the max of its highest_heard value and its own id.
+			        && var message := max(v.highest_heard[src], c.ids[src]);
+				    // dst only overwrites its highest_heard if the message is higher.
+				        && var dst_new_max := max(v.highest_heard[dst], message);
+					    // && v' == v.(highest_heard := v.highest_heard[dst := message])  // BUG: dst := dst_new_max
+					        && v' == v.(highest_heard := v.highest_heard[dst := dst_new_max])
+						}
 
 lemma test(c: Constants, v: Variables, src: nat) returns (v': Variables,w:Variables)
     // ensures !(LReplicaNextProcess2a(s, s', received_packet, sent_packets))
-// ensures !(Transmission(c,v,v',src))
-    // ensures !(Transmission(c,v,v',src) 
-    //           && v' != w
-    //           && Transmission(c,v,w,src))
-{
+    // ensures !(Transmission(c,v,v',src))
+        // ensures !(Transmission(c,v,v',src)
+	    //           && v' != w
+	        //           && Transmission(c,v,w,src))
+		{
 
 }
 
